fixed ext_invert with some admits in rule E_Pi

src/FcEtt/ext_invert.v
@@ -243,8 +243,8 @@ Proof.
   move e: (a_UAbs rho b0) => t1.
   move => h0.
   induction h0; auto; try done.
-  inversion e; subst.
-  - exists A, B, R.
+  inversion e; subst. Admitted.
+(*  - exists A, B, R.
     split.
     + inversion e; subst. apply (E_Refl _ _ _ a_Star); auto.
       apply (E_Pi (L \u (dom G))); auto.
@@ -262,114 +262,132 @@ Proof.
      split.
      + apply (@E_Trans _ _ _ _ _ A); auto.
      + split; auto.
-Qed.
+Qed. *)
 
 
-Lemma invert_a_UCAbs: forall G A b0,
-    Typing G (a_UCAbs b0) A ->
-    exists a b T B1, PropWff G (Eq a b T) /\ DefEq G (dom G) A (a_CPi (Eq a b T) B1) a_Star
-                /\ (exists L, forall c, c `notin` L ->
-                             Typing ([(c, Co (Eq a b T))] ++ G)
-                                    (open_tm_wrt_co b0 (g_Var_f c)) (open_tm_wrt_co B1 (g_Var_f c))
-                             /\ Typing ([(c, Co (Eq a b T))] ++ G) (open_tm_wrt_co B1 (g_Var_f c)) a_Star).
+Lemma invert_a_UCAbs: forall G A R b0,
+    Typing G (a_UCAbs b0) A R ->
+    exists a b T R' B1 R'', PropWff G (Eq a b T R')
+                /\ DefEq G (dom G) A (a_CPi (Eq a b T R') B1) a_Star R /\
+                (exists L, forall c, c `notin` L ->
+                           Typing ([(c, Co (Eq a b T R'))] ++ G)
+                                  (open_tm_wrt_co b0 (g_Var_f c))
+                                  (open_tm_wrt_co B1 (g_Var_f c)) R'' /\
+                           Typing ([(c, Co (Eq a b T R'))] ++ G)
+                                  (open_tm_wrt_co B1 (g_Var_f c)) a_Star R'')
+                 /\ SubRole R'' R.
 Proof.
-  intros G A b0.
+  intros G A R b0.
   move e: (a_UCAbs b0) => t1.
   move => h0.
   induction h0; auto; try done.
-  - destruct IHh0_1 as [a' [b' [T [B2 [h3 [h4 [L h5]]]]]]]; auto.
-    exists a', b', T, B2.
+  - destruct (IHh0 e) as 
+    [a' [b' [T [R' [B2 [R'' [h3 [h4 [h5 h6]]]]]]]]].
+    exists a', b', T, R', B2, R''. split; auto.
+    split. eapply E_Sub; eauto. split. apply h5. eauto.
+  - destruct IHh0_1 as
+    [a' [b' [T [R' [B2 [R'' [h3 [h4 [[L h5] h6]]]]]]]]]; auto.
+    exists a', b', T, R', B2, R''.
     split; auto.
     split.
-    + apply (E_Trans _ _ _ _ _ A); auto.
-    + exists L; auto.
+    + apply (E_Trans _ _ _ _ _ _ A); auto.
+    + split. exists L; auto. assumption.
   - induction phi.
-    exists a0, b, A, B.
+    exists a0, b, A, R0, B, R.
     split; auto.
     split.
     + apply (E_Refl _ _ _ a_Star); auto.
       apply (E_CPi (L \u (dom G))); auto.
       intros c H2.
       apply (@Typing_regularity (open_tm_wrt_co a (g_Var_f c))); auto.
-    + exists (L \u (dom G)).
+    + split. exists (L \u (dom G)).
       inversion e; subst; clear e.
       intros c H2.
       split; auto.
       apply (@Typing_regularity (open_tm_wrt_co a (g_Var_f c))); auto.
+      auto.
 Qed.
 
 
-Lemma invert_a_App_Rel : forall G a b C,
-    Typing G (a_App a Rel b) C ->
-    exists A B, Typing G a (a_Pi Rel A B) /\
-           Typing G b A /\
-           DefEq G (dom G) C (open_tm_wrt_tm B b) a_Star.
+Lemma invert_a_App_Rel : forall G a b C R,
+    Typing G (a_App a Rel b) C R ->
+    exists A B R1 R2, Typing G a (a_Pi Rel A R1 B) R2 /\
+           Typing G b A R1 /\
+           DefEq G (dom G) C (open_tm_wrt_tm B b) a_Star R /\ SubRole R2 R.
 Proof.
-  intros G a b C.
+  intros G a b C R.
   move e : (a_App a Rel b) => t1.
   move => h1.
   induction h1; auto; try done.
-  - exists A, B. inversion e; subst.
-    assert (h2 : Typing G (open_tm_wrt_tm B a0) a_Star).
-    + (have: Typing G (a_Pi Rel A B) a_Star by apply (Typing_regularity h1_1)) => h3.
+  - destruct (IHh1 e) as [A0 [B [R3 [R4 [h0 [h2 [h3 h4]]]]]]].
+    exists A0, B, R3, R4. repeat split; eauto 3.
+  - exists A, B, R, R'. inversion e; subst.
+    assert (h2 : Typing G (open_tm_wrt_tm B a0) a_Star R').
+    + (have: Typing G (a_Pi Rel A R B) a_Star R' by apply (Typing_regularity h1_1)) => h3.
       destruct (invert_a_Pi h3) as [_ [[L h4] h5]].
       pick fresh x.
       rewrite (tm_subst_tm_tm_intro x); auto.
       replace a_Star with (tm_subst_tm_tm a0 x a_Star); auto.
-      apply Typing_tm_subst with (A := A); auto.
+      apply Typing_tm_subst with (A := A) (R1 := R); auto.
     + repeat split; auto.
-  - destruct (IHh1_1 e) as [A0 [B0 [h3 [h2 e2]]]].
-    exists A0, B0.
+  - destruct (IHh1_1 e) as [A0 [B0 [R1 [R2 [h3 [h2 [e2 s]]]]]]].
+    exists A0, B0, R1, R2.
     repeat split; auto.
-    apply (E_Trans _ _ _ _ _ A); auto.
+    apply (E_Trans _ _ _ _ _ _ A); auto.
 Qed.
 
 
-Lemma invert_a_App_Irrel : forall G a b C,
-    Typing G (a_App a Irrel b) C ->
-    exists A B b0, Typing G a (a_Pi Irrel A B) /\
-              Typing G b0 A /\
-              DefEq G (dom G) C (open_tm_wrt_tm B b0) a_Star.
+Lemma invert_a_App_Irrel : forall G a b C R,
+    Typing G (a_App a Irrel b) C R ->
+    exists A B b0 R1 R2, Typing G a (a_Pi Irrel A R1 B) R2 /\
+              Typing G b0 A R1 /\
+              DefEq G (dom G) C (open_tm_wrt_tm B b0) a_Star R /\ SubRole R2 R.
 Proof.
-  intros G a b C.
+  intros G a b C R.
   move e : (a_App a Irrel b) => t1.
   move => h1.
   induction h1; auto; try done.
-  - exists A, B, a0. inversion e; subst.
-    assert (h2 : Typing G (open_tm_wrt_tm B a0) a_Star).
-    + (have: Typing G (a_Pi Irrel A B) a_Star by apply (Typing_regularity h1_1)) => h3.
+  - destruct (IHh1 e) as [A0 [B [b0 [R3 [R4 [h0 [h2 [h3 h4]]]]]]]].
+    exists A0, B, b0, R3, R4. repeat split; eauto 3.
+  - exists A, B, a0, R, R'. inversion e; subst.
+    assert (h2 : Typing G (open_tm_wrt_tm B a0) a_Star R').
+    + (have: Typing G (a_Pi Irrel A R B) a_Star R' by apply (Typing_regularity h1_1)) => h3.
       destruct (invert_a_Pi h3) as [_ [[L h4] h5]].
       pick fresh x.
       rewrite (tm_subst_tm_tm_intro x); auto.
       replace a_Star with (tm_subst_tm_tm a0 x a_Star); auto.
-      apply Typing_tm_subst with (A := A); auto.
+      apply Typing_tm_subst with (A := A) (R1 := R); auto.
     + repeat split; auto.
-  - destruct (IHh1_1 e) as [A0 [B0 [b0 [h3 [h2 h4]]]]].
-    exists A0, B0, b0.
+  - destruct (IHh1_1 e) as [A0 [B0 [b0 [R1 [R2 [h3 [h2 [h4 s]]]]]]]].
+    exists A0, B0, b0, R1, R2.
     repeat split; auto.
-    apply (E_Trans _ _ _ _ _ A); auto.
+    apply (E_Trans _ _ _ _ _ _ A); auto.
 Qed.
 
-Lemma invert_a_CApp : forall G a g A,
-    Typing G (a_CApp a g) A ->
+Lemma invert_a_CApp : forall G a g A R,
+    Typing G (a_CApp a g) A R ->
     g = g_Triv /\
-    exists a1 b1 A1 B, Typing G a (a_CPi (Eq a1 b1 A1) B) /\
-             DefEq G (dom G) a1 b1 A1 /\
-             DefEq G (dom G) A (open_tm_wrt_co B g_Triv) a_Star.
+    exists a1 b1 A1 R1 B R2, Typing G a (a_CPi (Eq a1 b1 A1 R1) B) R2 /\
+             DefEq G (dom G) a1 b1 A1 R1 /\
+             DefEq G (dom G) A (open_tm_wrt_co B g_Triv) a_Star R /\
+             SubRole R2 R.
 Proof.
-  intros G a g A H.
+  intros G a g A R H.
   dependent induction H.
-  - destruct (IHTyping1 a g) as (p & a1 & b1 & A1 & BB & Ta & Dab & DAB); first by done.
+  - destruct (IHTyping a g eq_refl) as (p & a1 & b1 & A1 & R3 & BB & R4 & Ta & Dab & DAB & s).
+    split; auto. exists a1, b1, A1, R3, BB, R4. repeat split; auto.
+    eapply E_Sub; eauto. eauto.
+  - destruct (IHTyping1 a g eq_refl) as (p & a1 & b1 & A1 & R3 & BB & R4 & Ta & Dab & DAB & s).
     split; first by done.
-    exists a1, b1, A1, BB.
+    exists a1, b1, A1, R3, BB, R4.
     repeat split; auto.
     apply E_Trans with (a1 := A); auto.
   - split; first by done.
-    exists a0, b, A, B1.
+    exists a0, b, A, R, B1, R'.
     repeat split; auto.
     eapply E_Refl.
     have CTX: Ctx G by eauto.
-    have TC: Typing G (a_CPi (Eq a0 b A) B1) a_Star. eapply Typing_regularity; eauto.
+    have TC: Typing G (a_CPi (Eq a0 b A R) B1) a_Star R'. eapply Typing_regularity; eauto.
     destruct (invert_a_CPi TC) as [_ [[L h4] h5]].
     pick fresh x.
     move: (h4 x ltac:(auto)) => h6.
@@ -383,11 +401,11 @@ Qed.
 
 Inductive context_DefEq : available_props -> context -> context -> Prop :=
 | Nul_Eqcontext: forall D, context_DefEq D nil nil
-| Factor_Eqcontext_tm: forall G1 G2 D A A' x,
+| Factor_Eqcontext_tm: forall G1 G2 D A A' R x,
     context_DefEq D G1 G2 ->
-    DefEq G1 D A A' a_Star ->
-    DefEq G2 D A A' a_Star ->
-    context_DefEq D ([(x, Tm A)] ++ G1) ([(x, Tm A')] ++ G2)
+    DefEq G1 D A A' a_Star R ->
+    DefEq G2 D A A' a_Star R ->
+    context_DefEq D ([(x, Tm A R)] ++ G1) ([(x, Tm A' R)] ++ G2)
 | Factor_Eqcontext_co: forall D G1 G2 Phi1 Phi2 c,
     context_DefEq D G1 G2 ->
     Iso G1 D Phi1 Phi2 ->
@@ -396,11 +414,11 @@ Inductive context_DefEq : available_props -> context -> context -> Prop :=
 
 Hint Constructors context_DefEq.
 
-Lemma context_tm_binding_defeq: forall D (G1 G2: context) A x,
+Lemma context_tm_binding_defeq: forall D (G1 G2: context) A R x,
     Ctx G1 -> Ctx G2 -> context_DefEq D G1 G2 ->
-    binds x (Tm A) G1 -> exists A', (binds x (Tm A') G2) /\ DefEq G2 D A A' a_Star.
+    binds x (Tm A R) G1 -> exists A', (binds x (Tm A' R) G2) /\ DefEq G2 D A A' a_Star R.
 Proof.
-  intros D G1 G2 A x H1 h0 H H0.
+  intros D G1 G2 A R x H1 h0 H H0.
   induction H; try done.
   - case H0; simpl.
     + intros M4.
@@ -409,7 +427,7 @@ Proof.
          -- left.
             inversion M4; auto.
          -- inversion M4; subst; clear M4.
-            rewrite_env (nil ++ [(x, Tm A')] ++ G2).
+            rewrite_env (nil ++ [(x, Tm A' R)] ++ G2).
             pose K := DefEq_weakening.
             inversion h0; subst.
             inversion H1; subst.
@@ -422,7 +440,7 @@ Proof.
       * intros A2 [h1 h2].
          exists A2.
          split; auto.
-         rewrite_env (nil ++ [(x0, Tm A')] ++ G2).
+         rewrite_env (nil ++ [(x0, Tm A' R0)] ++ G2).
          pose K := DefEq_weakening.
          eapply K; eauto.
   - case H0; try done; simpl.
@@ -477,7 +495,7 @@ Proof.
   induction 1.
   eauto.
   intros D' Sub.
-  pose K := (fourth weaken_available_mutual _ _ _ _ _ _ D' Sub). clearbody K.
+  pose K := (fourth weaken_available_mutual _ _ _ _ _ _ _ D' Sub). clearbody K.
   econstructor; eauto.
   intros D' Sub.
   pose K := (third weaken_available_mutual _ _ _ _ _ D' Sub). clearbody K.
@@ -491,14 +509,14 @@ Proof.
   simpl. rewrite IHcontext_DefEq. auto.
   simpl. rewrite IHcontext_DefEq. auto.
 Qed.
-
+ 
 
 Lemma context_DefEq_weaken_available :
   forall D G1 G2, context_DefEq D G1 G2 -> context_DefEq (dom G1) G1 G2.
 Proof.
   induction 1.
   eauto.
-  assert (SUB : (dom G1) [<=] (dom ([(x,Tm A)] ++ G1))). simpl. fsetdec.
+  assert (SUB : (dom G1) [<=] (dom ([(x,Tm A R)] ++ G1))). simpl. fsetdec.
   econstructor; auto.
   apply (context_DefEq_sub IHcontext_DefEq SUB).
   eapply (fourth weaken_available_mutual G1).
@@ -518,25 +536,25 @@ Qed.
 
 
 Lemma context_DefEq_mutual:
-  (forall G1  a A,   Typing G1 a A -> forall D G2,
-        Ctx G2 -> context_DefEq D G1 G2 -> Typing G2 a A) /\
+  (forall G1  a A R,   Typing G1 a A R -> forall D G2,
+        Ctx G2 -> context_DefEq D G1 G2 -> Typing G2 a A R) /\
   (forall G1  phi,   PropWff G1 phi -> forall D G2,
         Ctx G2 -> context_DefEq D G1 G2 -> PropWff G2 phi) /\
   (forall G1 D p1 p2, Iso G1 D p1 p2 ->
                   forall G2, Ctx G2 -> context_DefEq D G1 G2 -> Iso G2 D p1 p2) /\
-  (forall G1 D1 A B T,   DefEq G1 D1 A B T -> forall G2, Ctx G2 -> context_DefEq D1 G1 G2 ->
-                                          DefEq G2 D1 A B T) /\
-  (forall G1 ,       Ctx G1 -> forall G2 D x A, Ctx G2 -> context_DefEq D G1 G2
-                                   -> binds x (Tm A) G1 -> Typing G2 A a_Star).
+  (forall G1 D1 A B T R,   DefEq G1 D1 A B T R -> forall G2, Ctx G2 -> context_DefEq D1 G1 G2 ->
+                                          DefEq G2 D1 A B T R) /\
+  (forall G1 ,       Ctx G1 -> forall G2 D x A R, Ctx G2 -> context_DefEq D G1 G2
+                                   -> binds x (Tm A R) G1 -> Typing G2 A a_Star R).
 Proof.
   apply typing_wff_iso_defeq_mutual; eauto 3; try done.
-  - intros G1 x A c H b D G2 H0 H1.
-    case (@context_tm_binding_defeq D G1 G2 A x); auto.
+  - intros G1 x A R c H b D G2 H0 H1.
+    case (@context_tm_binding_defeq D G1 G2 A R x); auto.
     intros A2 [h0 h1].
-    apply (E_Conv _ _ _ A2); auto.
+    apply (E_Conv _ _ _ _ A2); auto.
     eapply DefEq_weaken_available; eauto.
     eapply H; eauto.
-  - intros L G1 rho A B t H t0 H0 D G2 H1 H2.
+  - intros L G1 rho A R B t H t0 H0 D G2 H1 H2.
     apply (E_Pi (L \u (dom G2))); auto.
     intros x H3.
     eapply H; auto.
@@ -544,7 +562,7 @@ Proof.
     apply Factor_Eqcontext_tm; eauto 2.
     eapply E_Refl; eauto.
     eapply H0; eauto.
-  - intros L G1 rho A a B t H t0 H0 r D G2 H1 H2.
+  - intros L G1 rho A a R B R' t H t0 H0 r S D G2 H1 H2.
     apply (E_Abs (L \u (dom G2))); auto.
     intros x H3.
     eapply H; auto.
@@ -553,13 +571,13 @@ Proof.
     eapply H0; eauto.
   - intros. eauto 4.
   - intros. eauto 4.
-  - intros G a B A t H d H0 d0 t0 D G2 H1 H2.
-    apply (E_Conv _ _ _ A); auto. eapply H; eauto.
+  - intros G a B R A t H d H0 d0 t0 D G2 H1 H2.
+    apply (E_Conv _ _ _ _ A); auto. eapply H; eauto.
     rewrite <- (same_dom H2).
     eapply H0; eauto.
     eapply context_DefEq_weaken_available. eauto.
     eapply t0; eauto.
-  - intros L G1 phi B t H p H0 D G2 H1 H2.
+  - intros L G1 phi B R t H p H0 D G2 H1 H2.
     apply (E_CPi (L \u (dom G2))); eauto.
     intros c H3.
     eapply H; eauto.
@@ -567,7 +585,7 @@ Proof.
     eapply refl_iso; auto.
     eapply refl_iso; auto.
     eauto.
-  - intros L G1 phi a B t H p H0 D G2 H1 H2.
+  - intros L G1 phi a B R t H p H0 D G2 H1 H2.
     apply (E_CAbs (L \u (dom G2))); auto.
     intros c H3.
     eapply H; eauto.
@@ -575,8 +593,8 @@ Proof.
     eapply refl_iso; eauto.
     eapply refl_iso; eauto.
     eauto.
-  - intros G a1 B1 a b A t H d H0 D G2 H1 H2.
-    apply (E_CApp _ _ _ a b A); auto. eauto.
+  - intros G a1 B1 R' a b A R t H d H0 D G2 H1 H2.
+    apply (E_CApp _ _ _ _ a b A R); auto. eauto.
     rewrite <- (same_dom H2).
     eapply H0. auto.
     eapply context_DefEq_weaken_available. eauto.
@@ -586,7 +604,7 @@ Proof.
     apply (E_Conv _ _ _ A'); eauto 2.
     apply E_Sym.
     eapply DefEq_weaken_available; eauto.
-  - *) intros G a b A t H t0 H0 t1 H1 D G2 H2 H3.
+  - *) intros G a b A R t H t0 H0 t1 H1 D G2 H2 H3.
     apply E_Wff; eauto.
   (*- intros G D A1 B1 A A2 B2 B d H d0 H0 d1 H1 G2 H2 H3.
     apply E_PropCong; auto.
@@ -594,10 +612,10 @@ Proof.
     eapply H1; auto.
     eapply context_DefEq_weaken_available. eauto.*)
   - intros. eauto 4.
-  - intros G D A1 A2 A B d H p H0 p0 H1 G2 H2 H3.
+  - intros G D A1 A2 A R B d H p H0 p0 H1 G2 H2 H3.
     eapply E_IsoConv; eauto.
-  - intros G D a b A c c0 H b0 i G2 H0 H1.
-    case (@context_co_binding_defeq D G G2 (Eq a b A) c); auto.
+  - intros G D a b A R c c0 H b0 i G2 H0 H1.
+    case (@context_co_binding_defeq D G G2 (Eq a b A R) c); auto.
     intros phi' [h0 h1].
     destruct phi' as [A' B'].
     eapply (E_Assn _ D) in h0; auto.
@@ -623,12 +641,12 @@ Proof.
     destruct phi1.
     eapply H; eauto.
     econstructor; eauto using refl_iso.
-  - intros G D a1 b1 B a b A d H d0 H0 G2 H1 H2.
+  - intros G D a1 b1 B R' a b A R d H d0 H0 G2 H1 H2.
     eapply E_CAppCong; eauto 2.
     rewrite <- (same_dom H2).
     apply H0; eauto.
     eapply context_DefEq_weaken_available. eauto.
-  - intros G D B1 B2 a1 a2 A a1' a2' A' d H d0 H0 d1 H1 G2 H2 H3.
+  - intros G D B1 B2 R0 a1 a2 A R a1' a2' A' R' d H d0 H0 d1 H1 G2 H2 H3.
     eapply E_CPiSnd; eauto 2. eapply DefEq_weaken_available.
     eapply H0; eauto 2.
     eapply context_DefEq_weaken_available. eauto 2.
@@ -636,44 +654,44 @@ Proof.
     eapply H1; eauto 2.
     eapply context_DefEq_weaken_available; eauto 2.
   - intros. eauto 4.
-  - intros G D a b B A d H d0 H0 G2 H1 H2.
-    apply (E_EqConv _ _ _ _ _ A); auto.
+  - intros G D a b B R2 A R1 d H d0 H0 S G2 H1 H2.
+    apply (E_EqConv _ _ _ _ _ _ A R1); auto.
     rewrite <- (same_dom H2).
     apply H0; auto.
     eapply context_DefEq_weaken_available; eauto.
-  - intros G x A c H t H0 n G2 D x0 A0 H1 H2 H3.
+  - intros G x A R c H t H0 n G2 D x0 A0 R' H1 H2 H3.
     inversion H3; subst.
     + inversion H4; subst.
       inversion H2; subst.
-      have: Typing G0 A0 a_Star; auto.
+      have: Typing G0 A0 a_Star R'; auto.
       * eapply H0; eauto.
       * move => h0.
         pose K := Typing_weakening.
-        rewrite_env (nil ++ [(x0, Tm A')] ++ G0).
-        apply (K _ _ _ h0); auto.
+        rewrite_env (nil ++ [(x0, Tm A' R')] ++ G0).
+        apply (K _ _ _ _ h0); auto.
     + inversion H2; subst.
-      have: Typing G0 A0 a_Star; auto.
+      have: Typing G0 A0 a_Star R'; auto.
       * apply (H _ D x0); auto.
           by inversion H1; auto.
       * move => h0.
         pose K := Typing_weakening.
-        rewrite_env (nil ++ [(x, Tm A')] ++ G0).
-        apply (K _ _ _ h0); auto.
-  - intros G c phi c0 H p H0 n G2 D x A H1 H2 H3.
+        rewrite_env (nil ++ [(x, Tm A' R)] ++ G0).
+        apply (K _ _ _ _ h0); auto.
+  - intros G c phi c0 H p H0 n G2 D x A R H1 H2 H3.
     inversion H3; try done.
     inversion H2; subst.
-    have: Typing G0 A a_Star.
+    have: Typing G0 A a_Star R.
     + apply (H _ D x); auto.
         by inversion H1.
     + move => h0.
       pose K := Typing_weakening.
       rewrite_env (nil ++ [(c, Co Phi2) ] ++ G0).
-      apply (K _ _ _ h0); auto.
+      apply (K _ _ _ _ h0); auto.
 Qed.
 
 Lemma context_DefEq_typing:
-  forall G1  a A,
-    Typing G1 a A -> forall D G2, Ctx G2 -> context_DefEq D G1 G2 -> Typing G2 a A.
+  forall G1  a A R,
+    Typing G1 a A R -> forall D G2, Ctx G2 -> context_DefEq D G1 G2 -> Typing G2 a A R.
 Proof.
   apply context_DefEq_mutual.
 Qed.
@@ -694,77 +712,81 @@ Qed.
 
 
 Lemma DefEqIso_regularity :
-  (forall G0 a A, Typing G0 a A -> True ) /\
+  (forall G0 a A R, Typing G0 a A R -> True ) /\
   (forall G0 phi,  PropWff G0 phi -> True ) /\
   (forall G D p1 p2, Iso G D p1 p2 ->
                  PropWff G p1 /\ PropWff G p2) /\
-  (forall G D A B T,   DefEq G D A B T ->
-                  Typing G A T /\ Typing G B T) /\
+  (forall G D A B T R,   DefEq G D A B T R ->
+                  Typing G A T R /\ Typing G B T R) /\
   (forall G0, Ctx G0 -> True).
 Proof.
   apply typing_wff_iso_defeq_mutual; eauto; try done.
-  - intros G D A1 B1 A A2 B2 d H d0 H0.
+  - intros G D A1 B1 A R A2 B2 d H d0 H0.
     split_hyp.
     split; apply E_Wff; solve [auto | eapply Typing_regularity; eauto].
-  - intros G D phi1 phi2 B1 B2 d H.
+  - intros G D phi1 phi2 B1 B2 R d H.
     split_hyp.
     have CTX: Ctx G by eauto.
     split; solve [eapply invert_a_CPi; eauto].
-  - intros G D a0 b0 A c c0 H b i.
+  - intros G D a0 b0 A R c c0 H b i.
     apply binds_to_PropWff in b; auto.
     inversion b; subst.
     split; auto.
-  -  intros G D a b A d H.
+  -  intros G D a b A R d H.
     split_hyp; auto.
-  - intros G D a b A a1 H1 H hi0 hi1.
+  - intros G D a b A R a1 H1 H hi0 hi1.
     destruct H as [h0 h1]; auto.
     split_hyp; auto.
-  - intros L G D rho b1 b2 A2 B d H0 t H1 r1 r2 .
+  - intros G D a b A R2 R1 d [T1 T2] S.
+    split; eapply E_SubRole; eauto.
+  - intros L G D rho b1 b2 A2 R B R' d H0 t H1 S r1 r2 .
     split_hyp.
     repeat split; auto.
     + apply (E_Abs (L \u (dom G))); eauto.
       intros x H4.
       apply H0; auto.
     + (have: Ctx G by eauto) => CTX.
-      apply (E_Conv _ _ _ ((a_Pi rho A2 B))); auto.
+      apply (E_Conv _ _ _ _ ((a_Pi rho A2 R B))); auto.
       -- apply (E_Abs (L \u dom G)); eauto.
          intros x H4.
-         eapply (@context_DefEq_typing ([(x, Tm A2)] ++ G)); eauto.
+         eapply (@context_DefEq_typing ([(x, Tm A2 R)] ++ G)); eauto.
          apply H0; auto.
          apply Factor_Eqcontext_tm; eauto.
          apply refl_context_defeq; auto.
       -- apply (E_PiCong (L \u (dom G))); auto.
          ++ intros x H4.
             apply E_Refl; eauto.
-            eapply (@context_DefEq_typing ([(x, Tm A2)] ++ G)); eauto.
+            eapply (@context_DefEq_typing ([(x, Tm A2 R)] ++ G)); eauto.
             eapply Typing_regularity; eauto 2.
             apply H0; auto.
             apply Factor_Eqcontext_tm; eauto.
             apply refl_context_defeq; auto.
-         ++ apply (E_Pi (L \u (dom G))); eauto.
+         ++ eapply E_SubRole. apply S.
+            apply (E_Pi (L \u (dom G))); eauto.
             intros x H4.
             have: x `notin` L; auto => h0.
             destruct (H0 x h0).
-            eapply Typing_regularity; eauto 2.
-         ++ apply (E_Pi (L \u (dom G))); eauto.
+            eapply Typing_regularity. eauto 2. admit.
+         ++ eapply E_SubRole. apply S.
+            apply (E_Pi (L \u (dom G))); eauto.
             intros x H4.
-            eapply Typing_regularity; eauto 2.
-            apply H0; eauto.
-      -- apply (E_Pi (L \u (dom G))); eauto.
+            eapply Typing_regularity; eauto 2. admit.
+            (*apply H0; eauto. *)
+      -- eapply E_SubRole. apply S. apply (E_Pi (L \u (dom G))); eauto.
          intros x H4.
          eapply Typing_regularity; eauto 2.
-         apply H0; eauto.
-  - intros G D a1 a2 b1 b2 B A d H d0 H0.
+         admit. (* apply H0; eauto. *)
+  - intros G D a1 a2 b1 b2 B R' A R d H d0 H0.
     split_hyp.
     (have: Ctx G by eauto) => CTX.
     split; eauto.
-    apply (E_Conv _ _ _ (open_tm_wrt_tm B b2)); auto.
+    apply (E_Conv _ _ _ _ (open_tm_wrt_tm B b2)); auto.
     eapply (E_App); eauto.
-    apply (E_PiSnd _ _ _ _ _ _ Rel A A); auto.
+    apply (E_PiSnd _ _ _ _ _ _ _ Rel A R A); auto.
     apply E_Refl; auto.
     eapply Typing_regularity; eauto.
     apply E_Sym.
-    eapply DefEq_weaken_available; eauto.
+    eapply DefEq_weaken_available. destruct R; eauto.
     apply Typing_regularity in H; auto.
     apply invert_a_Pi in H; eauto.
     destruct H as [_ [[L h0] _]].
@@ -776,18 +798,18 @@ Proof.
     simpl in K.
     destruct eq_dec; try congruence.
     rewrite tm_subst_tm_tm_fresh_eq in K; auto.
-  - intros G D A1 A2 B1 B2 d H h0 h1 _.
+  - intros G D A1 A2 B1 B2 R' d R H h0 h1 _.
     split_hyp.
     (have: Ctx G by eauto) => CTX.
     split; eauto.
-  - intros G D A1 A2 rho B1 B2 d H.
+  - intros G D A1 A2 R rho B1 B2 R' d H. 
     split_hyp.
     (have: Ctx G by eauto) => CTX.
+    apply E_PiFst in d.
     apply invert_a_Pi in H; eauto.
     apply invert_a_Pi in H0; eauto.
-    split_hyp.
-    split; eauto.
-  - intros G D B1 a1 B2 a2 rho A1 A2 d H d0 H0.
+    split_hyp; auto.
+  - intros G D B1 a1 B2 a2 R' rho A1 R A2 d H d0 H0.
     split_hyp.
     (have: Ctx G by eauto) => CTX.
     repeat split.
@@ -814,14 +836,14 @@ Proof.
       rewrite tm_subst_tm_tm_fresh_eq in K; auto.
       apply E_PiFst in d; auto.
       eapply DefEq_weaken_available; eauto.
-  - intros L G D a b phi1 B d H p H0.
+  - intros L G D a b phi1 B R d H p H0.
     split_hyp.
     have CTX: Ctx G by eauto.
     repeat split; eauto.
     + apply (E_CAbs (L \u (dom G))); eauto.
       intros c H3.
       apply H; eauto.
-    + apply (E_Conv _ _ _ ((a_CPi phi1 B))); auto.
+    + apply (E_Conv _ _ _ _ ((a_CPi phi1 B))); auto.
       * apply (E_CAbs (L \u (dom G))); eauto.
         intros c H3.
         eapply (@context_DefEq_typing ([(c, Co phi1)] ++ G)); eauto.
@@ -855,12 +877,12 @@ Proof.
         intros c H3.
         destruct (H c); auto.
         eapply Typing_regularity; eauto.
-  - intros L G D phi1 a phi2 b B i H d H0.
+  - intros L G D phi1 a R' phi2 b B R i H d H0.
     split_hyp.
     split.
     eapply E_CApp; eauto.
     eapply E_CApp; eauto.
-  - intros G D B1 B2 a1 a2 A a1' a2' A' d H d0 H0 d1 H1.
+  - intros G D B1 B2 R0 a1 a2 A R a1' a2' A' R' d H d0 H0 d1 H1.
     split_hyp.
     (have: Ctx G by eauto) => CTX.
     apply invert_a_CPi in H; auto.
@@ -883,26 +905,27 @@ Proof.
       simpl in K.
       destruct eq_dec; try congruence.
       rewrite co_subst_co_tm_fresh_eq in K; auto.
-  - intros G D a' b' A' a b A d H i H0.
+  - intros G D a' b' A' R' a b A R d H i H0.
     split_hyp.
     inversion H1; subst.
     (have: Ctx G by eauto) => h0.
     eauto.
-  - intros G D a b B A d H d0 H0.
+  - intros G D a b B R2 A R1 d H d0 H0 S.
     split_hyp; auto.
     split; eapply E_Conv; eauto.
-  - intros G D A A' a b a' b' i H.
+  - intros G D A A' a b R a' b' i H.
     split_hyp; eauto.
     inversion H0; subst.
     inversion H; subst.
     split; auto.
-    Unshelve. exact (dom G). exact (dom G). exact (dom G). exact (dom G). exact (dom G).
-Qed.
+    Unshelve. exact (dom G). exact (dom G).
+    auto. auto. auto. exact (dom G). exact (dom G). exact (dom G).
+Admitted.
 
 Lemma DefEq_regularity :
-  forall G D A B T, DefEq G D A B T -> PropWff G (Eq A B T).
+  forall G D A B T R, DefEq G D A B T R -> PropWff G (Eq A B T R).
 Proof.
-  intros G D A B T H.
+  intros G D A B T R H.
   apply DefEqIso_regularity in H.
   split_hyp.
   apply E_Wff; auto.
@@ -918,17 +941,17 @@ Qed.
 
 
 Lemma PropWff_regularity :
-  forall G A B T, PropWff G (Eq A B T) ->  Typing G A T /\ Typing  G B T.
+  forall G A B T R, PropWff G (Eq A B T R) ->  Typing G A T R /\ Typing  G B T R.
 Proof.
-  intros G A B T H.
+  intros G A B T R H.
   inversion H; subst.
   repeat split; auto.
 Qed.
 
 (* -------------------------------------------------------------- *)
 
-Lemma DefEq_conv : forall G D a b A B, DefEq G D a b A ->
-                                  DefEq G (dom G) A B a_Star -> DefEq G D a b B.
+Lemma DefEq_conv : forall G D a b A B R, DefEq G D a b A R -> 
+                  DefEq G (dom G) A B a_Star R -> DefEq G D a b B R.
 Proof.
   intros. eauto.
 Qed.
@@ -945,7 +968,7 @@ Proof.
 
   have CTX: Ctx G by eauto 2.
 
-  have DE1: DefEq G D (a_CPi (Eq a b A) a_Star) (a_CPi (Eq a0 b0 A0) a_Star) a_Star.
+  have DE1: DefEq G D (a_CPi (Eq a b A R) a_Star) (a_CPi (Eq a0 b0 A0 R0) a_Star) a_Star R.
   { pick fresh x and apply E_CPiCong; eauto 2.
     unfold open_tm_wrt_co. simpl.
     constructor. constructor. constructor; auto.
@@ -959,7 +982,7 @@ Proof.
     constructor. constructor; auto.
   }
 
-  have DE2: DefEq G D (a_CPi (Eq a0 b0 A0) a_Star) (a_CPi (Eq a2 b2 A2) a_Star) a_Star.
+  have DE2: DefEq G D (a_CPi (Eq a0 b0 A0 R0) a_Star) (a_CPi (Eq a2 b2 A2 R2) a_Star) a_Star R.
   { pick fresh x and apply E_CPiCong; eauto 2.
     unfold open_tm_wrt_co. simpl.
     constructor. constructor. constructor; auto.
@@ -973,33 +996,33 @@ Proof.
     constructor. constructor; auto.
   }
 
-  move: (E_Trans _ _ _ _ _ _ DE1 DE2) => DE3.
+  move: (E_Trans _ _ _ _ _ _ _ DE1 DE2) => DE3.
 
   eapply E_CPiFst. eauto.
 Qed.
 
-Lemma iso_cong : forall G D A A' B B' T T',
-    DefEq G D A A' T -> DefEq G D B B' T -> DefEq G D T T' a_Star ->
-    Iso G D (Eq A B T) (Eq A' B' T').
+Lemma iso_cong : forall G D A A' B B' T T' R, 
+                 DefEq G D A A' T R -> DefEq G D B B' T R -> 
+                 DefEq G D T T' a_Star R -> Iso G D (Eq A B T R) (Eq A' B' T' R).
     Proof.
       intros.
       move: (DefEq_regularity H) => p0. inversion p0.
       move: (DefEq_regularity H0) => p1. inversion p1.
       move: (DefEq_regularity H1) => p2. inversion p2.
       subst.
-      have AT: Typing G A T'.
+      have AT: Typing G A T' R.
       eapply E_Conv; eauto using DefEq_weaken_available.
-      have AT': Typing G A' T'.
+      have AT': Typing G A' T' R.
       eapply E_Conv; eauto using DefEq_weaken_available.
-      have BT: Typing G B T'.
+      have BT: Typing G B T' R.
       eapply E_Conv; eauto using DefEq_weaken_available.
-      have BT': Typing G B' T'.
+      have BT': Typing G B' T' R.
       eapply E_Conv; eauto using DefEq_weaken_available.
-      have IA: Iso G D (Eq A A' T) (Eq A A' T').
+      have IA: Iso G D (Eq A A' T R) (Eq A A' T' R).
       eapply E_IsoConv; eauto 2.
-      have IB: Iso G D (Eq B B' T) (Eq B B' T').
+      have IB: Iso G D (Eq B B' T R) (Eq B B' T' R).
       eapply E_IsoConv; eauto 2.
-      eapply trans_iso with (phi2 := Eq A B T').
+      eapply trans_iso with (phi2 := Eq A B T' R).
       eapply E_IsoConv; eauto.
       eapply E_PropCong; eauto 2.
     Qed.
@@ -1007,28 +1030,28 @@ Lemma iso_cong : forall G D A A' B B' T T',
 
 (* ----------------------------------------------------------------------------- *)
 
-Lemma E_PiCong2 :  ∀ (L : atoms) (G : context) (D : available_props) rho (A1 B1 A2 B2 : tm),
-    DefEq G D A1 A2 a_Star
+Lemma E_PiCong2 :  ∀ (L : atoms) (G : context) (D : available_props) rho (A1 B1 A2 B2 : tm) R,
+    DefEq G D A1 A2 a_Star R
     → (∀ x : atom,
           x `notin` L
-          → DefEq ([(x, Tm A1)] ++ G) D (open_tm_wrt_tm B1 (a_Var_f x))
-                  (open_tm_wrt_tm B2 (a_Var_f x)) a_Star)
-    → DefEq G D (a_Pi rho A1 B1) (a_Pi rho A2 B2) a_Star.
+          → DefEq ([(x, Tm A1 R)] ++ G) D (open_tm_wrt_tm B1 (a_Var_f x))
+                  (open_tm_wrt_tm B2 (a_Var_f x)) a_Star R)
+    → DefEq G D (a_Pi rho A1 R B1) (a_Pi rho A2 R B2) a_Star R.
 Proof.
   intros.
   move: (DefEq_regularity H) => WFF.
   inversion WFF. subst.
-  assert (Typing G A1 a_Star). eauto 1.
-  assert (Typing G (a_Pi rho A1 B1) a_Star).
+  assert (Typing G A1 a_Star R). eauto 1.
+  assert (Typing G (a_Pi rho A1 R B1) a_Star R).
   {  eapply (E_Pi L); eauto 1. intros x Fr.
      move: (DefEq_regularity (H0 x Fr)) => WFF2.
      inversion WFF2. subst. eauto 1. }
-  assert (Typing G (a_Pi rho A2 B2) a_Star).
+  assert (Typing G (a_Pi rho A2 R B2) a_Star R).
   {
      eapply (E_Pi L); eauto 1. intros x Fr.
      move: (DefEq_regularity (H0 x Fr)) => WFF2.
      inversion WFF2. subst.
-     have CTX: Ctx (x ~ Tm A1 ++ G) by eauto.
+     have CTX: Ctx (x ~ Tm A1 R ++ G) by eauto.
      inversion CTX. subst.
      eapply context_DefEq_typing; eauto 1.
      eapply E_ConsTm; eauto 1.
@@ -1038,27 +1061,26 @@ Proof.
 Qed.
 
 Lemma E_CPiCong2  : ∀ (L : atoms) (G : context) (D : available_props) (phi1 : constraint)
-                      (A : tm) (phi2 : constraint) (B : tm),
+                      (A : tm) (phi2 : constraint) (B : tm) R,
     Iso G D phi1 phi2
     → (∀ c : atom,
           c `notin` L
               → DefEq ([(c, Co phi1)] ++ G) D (open_tm_wrt_co A (g_Var_f c))
-                      (open_tm_wrt_co B (g_Var_f c)) a_Star)
-
-    → DefEq G D (a_CPi phi1 A) (a_CPi phi2 B) a_Star.
+                      (open_tm_wrt_co B (g_Var_f c)) a_Star R)
+    → DefEq G D (a_CPi phi1 A) (a_CPi phi2 B) a_Star R.
 Proof.
   intros.
   move: (Iso_regularity H) => [h0 h1].
   inversion h0. inversion h1. subst.
-  assert (Typing G (a_CPi (Eq a b A0) A) a_Star).
+  assert (Typing G (a_CPi (Eq a b A0 R0) A) a_Star R).
   { eapply (E_CPi L); eauto 1. intros x Fr.
     move: (DefEq_regularity (H0 x Fr)) => WFF2.
     inversion WFF2. subst. eauto 1. }
-  assert (Typing G (a_CPi (Eq a0 b0 A1) B) a_Star).
+  assert (Typing G (a_CPi (Eq a0 b0 A1 R1) B) a_Star R).
   { eapply (E_CPi L); eauto 1. intros x Fr.
     move: (DefEq_regularity (H0 x Fr)) => WFF2.
     inversion WFF2. subst.
-    have CTX: Ctx (x ~ Co (Eq a b A0) ++ G) by eauto.
+    have CTX: Ctx (x ~ Co (Eq a b A0 R0) ++ G) by eauto.
     inversion CTX. subst.
     eapply context_DefEq_typing; eauto 1.
     econstructor; eauto 1.
@@ -1070,35 +1092,36 @@ Qed.
 
 
 (* Could also be an exists form *)
-Lemma E_Pi2 : forall L G rho A B,
-    (∀ x : atom, x `notin` L → Typing ([(x, Tm A)] ++ G) (open_tm_wrt_tm B (a_Var_f x)) a_Star) ->
-    Typing G (a_Pi rho A B) a_Star.
+Lemma E_Pi2 : forall L G rho A B R,
+    (∀ x : atom, x `notin` L → Typing ([(x, Tm A R)] ++ G) (open_tm_wrt_tm B (a_Var_f x)) a_Star R) ->
+    Typing G (a_Pi rho A R B) a_Star R.
 Proof.
   intros.
   eapply E_Pi; eauto.
   pick fresh x.
   move: (H x ltac:(auto)) => h0.
-  have h1: Ctx (x ~ Tm A ++ G) by eauto.
+  have h1: Ctx (x ~ Tm A R ++ G) by eauto.
   inversion h1. auto.
 Qed.
 
-Lemma E_Abs2 : ∀ (L : atoms) (G : context) (rho : relflag) (a A B : tm),
+Lemma E_Abs2 : ∀ (L : atoms) (G : context) (rho : relflag) (a A B : tm) R R',
     (∀ x : atom,
-        x `notin` L → Typing ([(x, Tm A)] ++ G) (open_tm_wrt_tm a (a_Var_f x)) (open_tm_wrt_tm B (a_Var_f x)))
+        x `notin` L → Typing ([(x, Tm A R)] ++ G) (open_tm_wrt_tm a (a_Var_f x)) (open_tm_wrt_tm B (a_Var_f x)) R')
     → (∀ x : atom, x `notin` L → RhoCheck rho x (open_tm_wrt_tm a (a_Var_f x)))
-    → Typing G (a_UAbs rho a) (a_Pi rho A B).
+    -> SubRole R R'
+    → Typing G (a_UAbs rho a) (a_Pi rho A R B) R'.
 Proof.
   intros.
   eapply E_Abs; eauto.
   pick fresh x.
   move: (H x ltac:(auto)) => h0.
-  have h1: Ctx (x ~ Tm A ++ G) by eauto.
-  inversion h1. auto.
+  have h1: Ctx (x ~ Tm A R ++ G) by eauto.
+  inversion h1. auto. Unshelve. auto.
 Qed.
 
-Lemma E_Conv2 : ∀ (G : context) (a B A : tm),
-    Typing G a A → DefEq G (dom G) A B a_Star →
-    Typing G a B.
+Lemma E_Conv2 : ∀ (G : context) (a B A : tm) R,
+    Typing G a A R → DefEq G (dom G) A B a_Star R →
+    Typing G a B R.
 Proof.
   intros.
   eapply E_Conv; eauto.
@@ -1107,9 +1130,9 @@ Proof.
   auto.
 Qed.
 
-Lemma E_CPi2 :  ∀ (L : atoms) (G : context) (phi : constraint) (B : tm),
-    (∀ c : atom, c `notin` L → Typing ([(c, Co phi)] ++ G) (open_tm_wrt_co B (g_Var_f c)) a_Star) ->
-    Typing G (a_CPi phi B) a_Star.
+Lemma E_CPi2 :  ∀ (L : atoms) (G : context) (phi : constraint) (B : tm) R,
+    (∀ c : atom, c `notin` L → Typing ([(c, Co phi)] ++ G) (open_tm_wrt_co B (g_Var_f c)) a_Star R) ->
+    Typing G (a_CPi phi B) a_Star R.
 Proof.
   intros.
   eapply E_CPi; eauto.
@@ -1119,45 +1142,46 @@ Proof.
   inversion h1. auto.
 Qed.
 
-Lemma E_CAbs2 : ∀ (L : atoms) (G : context) (a : tm) (phi : constraint) (B : tm),
+Lemma E_CAbs2 : ∀ (L : atoms) (G : context) (a : tm) (phi : constraint) (B : tm) R,
        (∀ c : atom,
-        c `notin` L → Typing ([(c, Co phi)] ++ G) (open_tm_wrt_co a (g_Var_f c)) (open_tm_wrt_co B (g_Var_f c)))
-       → Typing G (a_UCAbs a) (a_CPi phi B).
+        c `notin` L → Typing ([(c, Co phi)] ++ G) (open_tm_wrt_co a (g_Var_f c)) (open_tm_wrt_co B (g_Var_f c)) R)
+       → Typing G (a_UCAbs a) (a_CPi phi B) R.
 Proof.
   intros.
   eapply E_CAbs; eauto.
   pick fresh x.
   move: (H x ltac:(auto)) => h0.
   have h1: Ctx (x ~ Co phi ++ G); eauto.
-  inversion h1. auto.
+  inversion h1. auto. Unshelve. auto.
 Qed.
 
 
 Lemma E_AbsCong2
-     : ∀ (L : atoms) (G : context) (D : available_props) (rho : relflag) (b1 b2 A1 B : tm),
+     : ∀ (L : atoms) (G : context) (D : available_props) (rho : relflag) (b1 b2 A1 B : tm) R R',
        (∀ x : atom,
         x `notin` L
-        → DefEq ([(x, Tm A1)] ++ G) D (open_tm_wrt_tm b1 (a_Var_f x)) (open_tm_wrt_tm b2 (a_Var_f x))
-            (open_tm_wrt_tm B (a_Var_f x)))
+        → DefEq ([(x, Tm A1 R)] ++ G) D (open_tm_wrt_tm b1 (a_Var_f x)) (open_tm_wrt_tm b2 (a_Var_f x))
+            (open_tm_wrt_tm B (a_Var_f x)) R')
        → (∀ x : atom, x `notin` L → RhoCheck rho x (open_tm_wrt_tm b1 (a_Var_f x)))
        → (∀ x : atom, x `notin` L → RhoCheck rho x (open_tm_wrt_tm b2 (a_Var_f x)))
-       → DefEq G D (a_UAbs rho b1) (a_UAbs rho b2) (a_Pi rho A1 B).
+       -> SubRole R R'
+       → DefEq G D (a_UAbs rho b1) (a_UAbs rho b2) (a_Pi rho A1 R B) R'.
 Proof.
   intros.
   eapply E_AbsCong; eauto.
   pick fresh x.
   move: (H x ltac:(auto)) => h0.
-  have h1: Ctx (x ~ Tm A1 ++ G) by eauto.
+  have h1: Ctx (x ~ Tm A1 R ++ G) by eauto.
   inversion h1; auto.
 Qed.
 
 Lemma E_CAbsCong2
-     : ∀ (L : atoms) (G : context) (D : available_props) (a b : tm) (phi1 : constraint)
+     : ∀ (L : atoms) (G : context) (D : available_props) (a b : tm) (phi1 : constraint) R
        (B : tm),
        (∀ c : atom,
         c `notin` L
         → DefEq ([(c, Co phi1)] ++ G) D (open_tm_wrt_co a (g_Var_f c)) (open_tm_wrt_co b (g_Var_f c))
-                (open_tm_wrt_co B (g_Var_f c))) → DefEq G D (a_UCAbs a) (a_UCAbs b) (a_CPi phi1 B).
+                (open_tm_wrt_co B (g_Var_f c)) R) → DefEq G D (a_UCAbs a) (a_UCAbs b) (a_CPi phi1 B) R.
 Proof.
   intros.
   eapply E_CAbsCong; eauto.
@@ -1167,9 +1191,9 @@ Proof.
   inversion h1. auto.
 Qed.
 
-Lemma E_Fam2 : ∀ (G : context) (F : tyfam) (A a : tm),
+Lemma E_Fam2 : ∀ (G : context) (F : tyfam) (A a : tm) R,
        Ctx G
-       → binds F (Ax a A) toplevel → Typing G (a_Fam F) A.
+       → binds F (Ax a A R) toplevel → Typing G (a_Fam F) A R.
 Proof.
   intros.
   eapply E_Fam; eauto.
@@ -1178,7 +1202,7 @@ Proof.
 Qed.
 
 
-Lemma E_Wff2 : ∀ (G : context) (a b A : tm), Typing G a A → Typing G b A → PropWff G (Eq a b A).
+Lemma E_Wff2 : ∀ (G : context) (a b A : tm) R, Typing G a A R → Typing G b A R → PropWff G (Eq a b A R).
 Proof.
   intros.
   eapply E_Wff; eauto.
